src/basic/FStarC.Errors.Codes.fst
@@ -382,4 +382,5 @@ let default_settings : list error_setting =
     Error_CustardUnextractableEffect                  , CAlwaysError, 365;
     Warning_CustardLostRepresentation                 , CWarning, 366;
     Error_CustardNoCRepresentation                    , CAlwaysError, 367;
+    Error_CustardBadUnitInterface                     , CAlwaysError, 368;
     ]
